coq/README.md
@@ -4,30 +4,3 @@ This directory is intended as a formal-basis for the implementations in the rest
 While it is unlikely I will feel compelled to extract the computable functions to **`OCaml`** or **`Haskell`**,
 the implementations here will at least provide some (informal) assurances of the correctness of
 my other implementations, which will be (mostly) identical to the code found here.
-
-## Monomorphic Type-Inference
-
-This is a simply-typed lambda-caluclus extended with numeric & boolean arithmetic.
-The syntax is given in ***Curry-style***, i.e. w/o type-annotations given in term-abstractions.
-
-Here are formal definitions of constraint generation and unification as described in
-[Types and Programming Languages](https://www.cis.upenn.edu/~bcpierce/tapl/),
-as well as corresponding computable functions.
-
-The constraint generation rules are defined in
-reference to a declarative typing semantics, and should be "equivalent".
-
-### Proven Results
-
-- Soundness of constraint generation with respect to declarative typing (`Mono.v`).
-- Soundness of computable constraint generation
-with respect to the ***`Inductive`*** definition (`MonoComputable.v`).
-- Termitation of the unification algorithm (`Unify.v`).
-
-### In Progress
-
-Completeness results have proved much more elusive than their soundness counterparts.
-- Completeness of constraint generation with respect to declarative typing (`MonoCompleteness.v`).
-- Completeness of computable constraint generation
-with respect to the ***`Inductive`*** definition (`MonoComputable.v`).
-- Adding `let` expressions to the language, albeit w/o ***`let`-polymorphism***.
